finalize case ticket13

src/tls/Parsers.Ticket.Low.fst
@@ -132,3 +132,47 @@ let finalize_case_ticketContents12 input pos =
   in
   [@inline_let] let _ = assert_norm (LP.parse_sum_kind (LP.get_parser_kind ticketVersion_repr_parser) ticketContents_sum parse_ticketContents_cases == ticketContents_parser_kind) in
   jump_ticketContents12 input pos1
+
+#reset-options "--max_fuel 0 --max_ifuel 0 --z3rlimit 16 --print_z3_statistics"
+
+inline_for_extraction
+let jump_ticketContents13 : LP.jumper ticketContents13_parser =
+  assert_norm (ticketContents13' == LP.get_parser_type (
+    cipherSuite_parser
+    `LP.nondep_then` ticketContents13_rms_parser
+    `LP.nondep_then` ticketContents13_nonce_parser
+    `LP.nondep_then` LP.parse_u32
+    `LP.nondep_then` LP.parse_u32
+    `LP.nondep_then` ticketContents13_custom_data_parser
+  )); // because of refinements
+  synth_ticketContents13_injective ();
+  LP.jump_synth
+    (LP.jump_constant_size cipherSuite_parser 2ul ()
+    `LP.jump_nondep_then`
+    LP.jump_bounded_vlbytes 32 255
+    `LP.jump_nondep_then`
+    LP.jump_bounded_vlbytes 0 255
+    `LP.jump_nondep_then`
+    LP.jump_u32
+    `LP.jump_nondep_then`
+    LP.jump_u32
+    `LP.jump_nondep_then`
+    LP.jump_bounded_vlbytes 0 65535)
+    synth_ticketContents13
+    ()
+
+#reset-options "--z3rlimit 16 --z3cliopt smt.arith.nl=false --max_fuel 0 --max_ifuel 0 --print_z3_statistics --z3refresh --using_facts_from '* -Parsers +Parsers.Ticket.Low +Parsers.TicketContents13 +Parsers.TicketVersion +Parsers.TicketContents -LowParse +LowParse.Spec.Base +LowParse.Low.Base +LowParse.Spec.Combinators +LowParse.Spec.Enum +LowParse.Spec.Sum +LowParse.Low.Sum -FStar.Tactics -FStar.Reflection' --print_implicits"
+
+let finalize_case_ticketContents13 input pos =
+  [@inline_let] let _ =
+    assert_norm (LP.list_mem Ticket13 (LP.list_map fst ticketVersion_enum) == true);
+    assert_norm ((LP.get_parser_kind parse_ticketVersion_key).LP.parser_kind_low == 1);
+    assert_norm ((LP.get_parser_kind parse_ticketVersion_key).LP.parser_kind_high == Some 1)
+  in
+  let pos1 = write_ticketVersion_key Ticket13 input pos in
+  let h = HST.get () in
+  [@inline_let] let _ =
+    LP.valid_sum_intro h ticketContents_sum ticketVersion_repr_parser parse_ticketContents_cases input pos
+  in
+  [@inline_let] let _ = assert_norm (LP.parse_sum_kind (LP.get_parser_kind ticketVersion_repr_parser) ticketContents_sum parse_ticketContents_cases == ticketContents_parser_kind) in
+  jump_ticketContents13 input pos1
